Specify length of generated Low* test vectors and make them recallable; verify Test.Bytes; use null instead of alloca 0uy and partially verify Test

providers/test/Test.fst
@@ -4,11 +4,7 @@ module G = FStar.Ghost
 module B = LowStar.Buffer
 module U32 = FStar.UInt32
 
-
-module T = LowStar.ToFStarBuffer
-
 open FStar.HyperStack.ST
-open FStar.Bytes
 open EverCrypt.Helpers
 
 module AC = EverCrypt.AutoConfig
@@ -16,81 +12,125 @@ module H = EverCrypt.Hash
 
 open Test.Vectors
 open LowStar.BufferOps
+open C.Failure
 
-#set-options "--admit_smt_queries true"
+open Test.Lowstarize
+
+#reset-options "--z3rlimit 50 --max_fuel 1 --max_ifuel 0 --using_facts_from '* -Test.Vectors'"
 
 /// Hash function (any of them)
 
-let vec8 = B.buffer UInt8.t * UInt32.t
+let vec8 = lbuffer UInt8.t
 let hash_vector = hash_alg * C.String.t * vec8 * UInt32.t
 
-noextract unfold inline_for_extraction let (!$) = C.String.((!$))
-
-open C.Failure
+noextract unfold inline_for_extraction
+let (!$) = C.String.((!$))
 
 let supported_hash_algorithm = function
   | H.SHA256 | H.SHA384 -> true
   | _ -> false
 
-val test_one_hash: hash_vector -> St unit
+val compute:
+  a: EverCrypt.Hash.alg ->
+  len: UInt32.t ->
+  text: uint8_pl (U32.v len) ->
+  tag: uint8_pl (EverCrypt.Hash.tagLength (Ghost.hide a)) -> ST unit
+  (requires fun h0 ->
+    B.live h0 text /\
+    B.live h0 tag /\
+    B.(loc_disjoint (loc_buffer text) (loc_buffer tag)))
+  (ensures fun h0 () h1 ->
+    B.live h1 text /\ B.live h1 tag /\
+    //B.modifies (B.loc_buffer tag) h0 h1 /\
+    U32.v len <= EverCrypt.Hash.maxLength (Ghost.hide a) /\ (* required for subtyping the RHS below *)
+    B.as_seq h1 tag = EverCrypt.Hash.spec (Ghost.hide a) (B.as_seq h0 text))
+//18-07-07 CF: TODO add deallocation; restore Stack (not ST); restore modifies clause
+let compute a len text tag =
+  let open FStar.Integers in
+  let open FStar.HyperStack.ST in
+  let open EverCrypt.Hash in
+  push_frame();
+  let s = create a in
+  assert_norm(U32.v len <= maxLength (Ghost.hide a));
+  let ll = len % blockLen a in
+  let lb = len - ll in
+  let blocks = B.sub text 0ul lb in
+  let last = B.offset text lb in
+  let h1 = get() in
+  init s;
+  let h10 = get() in
+  update_multi (Ghost.hide Seq.empty) s blocks lb;
+  let h11 = get() in
+  //18-07-10 CF: improve style on ghosts and lists?
+  FStar.Seq.(lemma_eq_intro (empty @| (B.as_seq h10 blocks)) (B.as_seq h10 blocks));
+  update_last (Ghost.hide (B.as_seq h11 blocks)) s last len;
+  finish s tag;
+  let h2 = get() in
+  pop_frame();
+
+  let vblocks = B.as_seq h1 blocks in
+  let vlast = B.as_seq h1 last in
+  let vsuffix = suffix (Ghost.hide a) (U32.v len) in
+  FStar.Seq.(lemma_eq_intro (B.as_seq h1 text) (vblocks @| vlast));
+  lemma_hash2 (acc0 #(Ghost.hide a)) vblocks FStar.Seq.(vlast @| vsuffix);
+  Seq.append_assoc vblocks vlast vsuffix
+
+#set-options "--max_fuel 0"
+
+val test_one_hash: hash_vector -> ST unit
+  (requires fun _ -> True)
+  (ensures  fun h0 _ h1 -> True)
 let test_one_hash vec =
   let open FStar.Integers in
-  let a, input, (expected, expected_len), repeat = vec in
-
-  if supported_hash_algorithm a then (
-
+  let a, input, (LB expected_len expected), repeat = vec in
+  if supported_hash_algorithm a then
+    begin
     push_frame();
-    let tlen: UInt32.t = H.tagLen a in
-// to avoid double-extraction of failwith
-//  let expected: uint8_pl (v tlen) =
-//    if expected_len = tlen
-//    then expected
-//    else failwith !$"Wrong output length" in
+    let tlen = H.tagLen a in
     let computed = B.alloca 0uy tlen in
-
     let input_len = C.String.strlen input in
+    assume (v input_len * v repeat < pow2 32);
     let total_input_len = input_len * repeat in
-    let total_input = B.alloca 0uy total_input_len in
-    C.Loops.for 0ul repeat (fun _ _ -> True) (fun i ->
-      C.String.memcpy (B.offset total_input (input_len * i)) input input_len
-    );
+    if total_input_len = 0ul then
+      begin
+      let total_input = B.null in
+      assert_norm (v total_input_len <= EverCrypt.Hash.maxLength (Ghost.hide a));
 
-    //18-08-03  this duplicated code now verified in EverCrypt.Hash.Test (and was a bit out of date)
-    (*
-    (* Allocate memory for state *)
-    let ctx = EverCrypt.Hash.create a in
-
-    (* Compute the number of blocks to process *)
-    let size_block: UInt32.t = H.blockLen a in
-    let n = U32.div total_input_len size_block in
-    let r = U32.rem total_input_len size_block in
-
-    (* Get all full blocks and the last block *)
-    let input_blocks = B.sub total_input 0ul (n * size_block) in
-    let input_last   = B.sub total_input (n * size_block) r in
-
-    (* Call the hash function incrementally *)
-    EverCrypt.Hash.init ctx;
-    EverCrypt.Hash.update_multi (G.hide Seq.empty) ctx input_blocks n;
-    EverCrypt.Hash.update_last (G.hide Seq.empty) ctx input_last r;
-    EverCrypt.Hash.finish ctx computed;
-    *)
-
-    let str: C.String.t = H.string_of_alg a in
-
-    //18-08-03 scopes?!!
-    // Incrementally:
-    // EverCrypt.Hash.Test.compute a input_len input computed;
-    // TestLib.compare_and_print str expected computed tlen;
-
-    // Non-incrementally:
-    if AC.(sha256_impl () = Vale) then
-      EverCrypt.Hash.Test.compute a total_input_len total_input computed
+      if AC.(sha256_impl () = Vale) then
+        compute a total_input_len total_input computed
+      else
+        EverCrypt.Hash.hash a computed total_input total_input_len
+      end
     else
-      EverCrypt.Hash.hash a computed total_input total_input_len;
+      begin
+      push_frame();
+      let total_input = B.alloca 0uy total_input_len in
+      let h0 = get () in
+      C.Loops.for 0ul repeat
+      (fun h i -> B.live h total_input /\ B.modifies (B.loc_buffer total_input) h0 h)
+      (fun i ->
+        assert (v input_len * v i + v input_len <= v input_len * (v repeat - 1) + v input_len);
+        assert (v input_len * v i + v input_len <= v input_len * v repeat);
+        C.String.memcpy (B.sub total_input (input_len * i) input_len) input input_len
+      );
+      assert_norm (v total_input_len <= EverCrypt.Hash.maxLength (Ghost.hide a));
+
+      if AC.(sha256_impl () = Vale) then
+        compute a total_input_len total_input computed
+      else
+        EverCrypt.Hash.hash a computed total_input total_input_len;
+      pop_frame()
+      end;
+
+    B.recall expected;
+    assume (expected_len == tlen);
+    let str = H.string_of_alg a in
     TestLib.compare_and_print str expected computed tlen;
     pop_frame()
-  )
+    end
+
+// 2018.08.06 SZ: TODO: verify the rest of the file
+#set-options "--admit_smt_queries true"
 
 /// HMAC
 
@@ -99,24 +139,21 @@ let hmac_vector = hash_alg * vec8 * vec8 * vec8
 val test_one_hmac: hmac_vector -> St unit
 let test_one_hmac vec =
   let open FStar.Integers in
-  let ha, (key,keylen), (data,datalen), (expected,expectedlen) = vec in
-
-  if supported_hash_algorithm ha then (
-
+  let ha, (LB keylen key), (LB datalen data), (LB expectedlen expected) = vec in
+  if supported_hash_algorithm ha then
+    begin
     push_frame();
 //  if expectedlen <> H.tagLen ha then failwith !$"Wrong output length"; 
     let computed = B.alloca 0uy (H.tagLen ha) in
     let str = EverCrypt.Hash.string_of_alg ha  in
     EverCrypt.HMAC.compute ha computed key keylen data datalen;
     TestLib.compare_and_print str expected computed (H.tagLen ha);
-
-    pop_frame() )
+    pop_frame()
+    end
 
 val test_hmac: len:U32.t -> vs: B.buffer hmac_vector {B.len vs = len } -> St unit
 let rec test_hmac len vs =
-
   C.String.print !$"HMAC\n";
-
   let open FStar.Integers in
   if len > 0ul then
     let v = vs.(0ul) in
@@ -130,14 +167,12 @@ let hkdf_vector = hash_alg * vec8 * vec8 * vec8 * vec8 * vec8
 val test_one_hkdf: hkdf_vector -> St unit
 let test_one_hkdf vec =
   let open FStar.Integers in
-  let ha, (ikm,ikmlen), (salt,saltlen), (info,infolen), (expected_prk,prklen), (expected_okm,okmlen) = vec in
+  let ha, (LB ikmlen ikm), (LB saltlen salt), (LB infolen info), (LB prklen expected_prk), (LB okmlen expected_okm) = vec in
 
-  if supported_hash_algorithm ha then (
-
+  if supported_hash_algorithm ha then
+    begin
     push_frame();
-
     // TODO test vector length validation
-
     let str = EverCrypt.Hash.string_of_alg ha  in 
     let computed_prk = B.alloca 0uy (H.tagLen ha) in
     EverCrypt.HKDF.hkdf_extract ha computed_prk salt saltlen ikm ikmlen;
@@ -146,10 +181,10 @@ let test_one_hkdf vec =
     let computed_okm = B.alloca 0uy okmlen in
     EverCrypt.HKDF.hkdf_expand ha computed_okm computed_prk prklen info infolen okmlen;
     TestLib.compare_and_print str expected_okm computed_okm okmlen;
+    pop_frame()
+    end
 
-    pop_frame() )
-
-val test_hkdf: len:U32.t -> vs: B.buffer hkdf_vector {B.len vs = len } -> St unit
+val test_hkdf: len:U32.t -> vs: B.buffer hkdf_vector {B.len vs == len} -> St unit
 let rec test_hkdf len vs =
   C.String.print !$"HKDF\n";
   let open FStar.Integers in
@@ -157,7 +192,6 @@ let rec test_hkdf len vs =
     let v = vs.(0ul) in
     test_one_hkdf v;
     test_hkdf (len - 1ul) (B.offset vs 1ul)
-
 
 /// ChaCha20-Poly1305
 
@@ -167,10 +201,9 @@ val test_chacha20_poly1305: aead_vector -> St unit
 let test_chacha20_poly1305 vec =
   push_frame();
 
-  let cipher, (key, key_len), (iv, iv_len), (aad, aad_len),
-    (tag, tag_len), (plaintext, plaintext_len), (ciphertext, ciphertext_len) = vec
+  let cipher, (LB key_len key), (LB iv_len iv), (LB aad_len aad),
+    (LB tag_len tag), (LB plaintext_len plaintext), (LB ciphertext_len ciphertext) = vec
   in
-
   let plaintext'    = B.alloca 0uy plaintext_len in
   let ciphertext'   = B.alloca 0uy plaintext_len in
   let tag'          = B.alloca 0uy 16ul in
@@ -194,8 +227,8 @@ val test_aes128_gcm: v:aead_vector -> St unit
 let test_aes128_gcm vec =
   push_frame();
 
-  let cipher, (key, key_len), (iv, iv_len), (aad, aad_len),
-    (tag, tag_len), (plaintext, plaintext_len), (ciphertext, ciphertext_len) = vec
+  let cipher, (LB key_len key), (LB iv_len iv), (LB aad_len aad),
+    (LB tag_len tag), (LB plaintext_len plaintext), (LB ciphertext_len ciphertext) = vec
   in
 
   let plaintext'    = B.alloca 0uy plaintext_len in
@@ -221,8 +254,8 @@ val test_aes256_gcm: v:aead_vector -> St unit
 let test_aes256_gcm vec =
   push_frame();
 
-  let cipher, (key, key_len), (iv, iv_len), (aad, aad_len),
-    (tag, tag_len), (plaintext, plaintext_len), (ciphertext, ciphertext_len) = vec
+  let cipher, (LB key_len key), (LB iv_len iv), (LB aad_len aad),
+    (LB tag_len tag), (LB plaintext_len plaintext), (LB ciphertext_len ciphertext) = vec
   in
 
   let plaintext'    = B.alloca 0uy plaintext_len in
@@ -253,7 +286,7 @@ type block_cipher_vector = block_cipher * vec8 * vec8 * vec8
 
 let test_aes_ecb (v: block_cipher_vector) : St unit =
   push_frame();
-  let block, (key, key_len), (plain, plain_len), (cipher, cipher_len) = v in
+  let block, (LB key_len key), (LB plain_len plain), (LB cipher_len cipher) = v in
   let cipher' = B.alloca 0uy 16ul in
   let s0 = TestLib.cpucycles () in
   let () =
@@ -287,7 +320,7 @@ let rec test_chacha20 (len: U32.t) (vs: B.buffer chacha20_vector): St unit =
   let open FStar.Integers in
   if len > 0ul then begin
     push_frame ();
-    let (key, key_len), (iv, iv_len), ctr, (plain, plain_len), (cipher, cipher_len) = vs.(0ul) in
+    let (LB key_len key), (LB iv_len iv), ctr, (LB plain_len plain), (LB cipher_len cipher) = vs.(0ul) in
     let cipher' = B.alloca 0uy cipher_len in
     EverCrypt.chacha20 key iv ctr plain plain_len cipher';
     TestLib.compare_and_print !$"of ChaCha20 message" cipher cipher' cipher_len;
@@ -295,7 +328,7 @@ let rec test_chacha20 (len: U32.t) (vs: B.buffer chacha20_vector): St unit =
     test_chacha20 (len - 1ul) (B.offset vs 1ul)
   end
 
-val test_aead: len:U32.t -> vs: B.buffer aead_vector {B.len vs = len }-> St unit
+val test_aead: len:U32.t -> vs: B.buffer aead_vector {B.len vs == len} -> St unit
 let rec test_aead len vs =
   if len = 0ul then
     ()
@@ -314,7 +347,7 @@ let rec test_aead len vs =
     let open FStar.Integers in
     test_aead (len - 1ul) (B.offset vs 1ul)
 
-val test_hash: len:U32.t -> vs: B.buffer hash_vector {B.len vs = len }-> St unit
+val test_hash: len:U32.t -> vs: B.buffer hash_vector{B.len vs == len} -> St unit
 let rec test_hash len vs =
   let open FStar.Integers in
   if len > 0ul then
@@ -327,12 +360,12 @@ let main (): St C.exit_code =
   let open C.String in
   push_frame ();
 
-  let hash_vectors, hash_vectors_len = hash_vectors_low in
-  let hmac_vectors, hmac_vectors_len = hmac_vectors_low in
-  let hkdf_vectors, hkdf_vectors_len = hkdf_vectors_low in
-  let aead_vectors, aead_vectors_len = aead_vectors_low in
-  let block_cipher_vectors, block_cipher_vectors_len = block_cipher_vectors_low in
-  let chacha20_vectors, chacha20_vectors_len = chacha20_vectors_low in
+  let LB hash_vectors_len hash_vectors = hash_vectors_low in
+  let LB hmac_vectors_len hmac_vectors = hmac_vectors_low in
+  let LB hkdf_vectors_len hkdf_vectors = hkdf_vectors_low in
+  let LB aead_vectors_len aead_vectors = aead_vectors_low in
+  let LB block_cipher_vectors_len block_cipher_vectors = block_cipher_vectors_low in
+  let LB chacha20_vectors_len chacha20_vectors = chacha20_vectors_low in
 
   print !$"===========Hacl===========\n";
   AC.(init (Prefer Hacl));
